a lot of cleanup of the file

rocq-brick-libcpp/proof/shared_ptr/specs.v
@@ -7,23 +7,10 @@ Require Import bluerock.cpp.stdlib.algorithms.spec.
 Require Import bluerock.cpp.stdlib.new.spec_exc.
 Require Import bluerock.brick.libcpp.newarr.spec_exc.
 Require Import bluerock.brick.libcpp.newarr.hints.
+Require Import bluerock.brick.libcpp.newarr.test. (* TODO move [dynAllocatedR] to a non-test file *)
 Require Import bluerock.cpp.spec.concepts.
 Require Import bluerock.cpp.spec.concepts.experimental.
 Require Import bluerock.brick.libcpp.shared_ptr.inc_shared_ptr_cpp.
-Lemma seqprefix (prelen len start: nat):
-  (prelen <= len)%nat -> seq start len = (seq start prelen)++(seq (start+prelen) (len -prelen)).
-Proof using.
-  intros Hl.
-  replace len with (prelen+(len-prelen))%nat at 1 by lia.
-  rewrite seq_app.
-  reflexivity.
-Qed.
-
-Definition liftQ {PROP: bi} (p: Qp->PROP) (q:Q) : PROP :=
-  match toQp q with
-  | None => emp
-  | Some qp => p qp
-  end.
 
 Record CtrlBlockId : Set :=
   {
@@ -42,30 +29,18 @@ Definition ctrlBlockPtrOffset: offset. Proof. Admitted.
 
 Lemma maxContentionLb : 2^32 <= Npos maxContention. Proof. Admitted.
 Definition maxContentionQp := pos_to_Qp maxContention.
+Definition allContenderIds : list nat := (seq 0 (Pos.to_nat maxContention)).
+Definition allButFirstContenderId := (seq 1 (Pos.to_nat maxContention -1 )).
 
 Definition countLN {A : Type} (f : A -> bool) (l : list A) : N :=
   lengthN (filter f l).
 
-
 Section specs.
-  Context `{Σ : cpp_logic, MOD:inc_shared_ptr_cpp.module ⊧ σ}.
+  Context `{Σ : cpp_logic, MOD:inc_shared_ptr_cpp.module ⊧ σ}
+  {hf:fracG () _Σ} (ty:type).
 
   Import linearity.
 
-  (* TODO: dedup from newarr/test.v *)
-  Definition dynAllocatedR ty (base:ptr) : mpred :=
-    Exists (bookKeepingLoc:ptr) (overhead:N),
-      match (size_of _ ty) with
-      | Some sz => bookKeepingLoc |-> pred.allocatedR 1 (overhead+sz)
-      | None => False
-      end
-      **  (base |-> new_token.R 1
-                {| new_token.alloc_ty := ty;
-                   new_token.storage_ptr := bookKeepingLoc.["unsigned char" ! overhead];
-                   new_token.overhead := overhead |}).
-
-
-  Context {hf:fracG () _Σ}.
 
   (* just an execlusive token for each contenderid. can be defined with a simpler CMRA as fractionality is not needed. fgptsoQ has good automation support  *)
   Definition copyConstrRight ctrlid contenderid : mpred :=
@@ -74,15 +49,14 @@ Section specs.
     | None => emp (* bad argument, contenderid > maxContention *)
     end.
       
-  Definition allContenderIds : list nat := (seq 0 (Pos.to_nat maxContention)).
   
   (** Currently, we assume the control block is just an atomic counter.
       In reality, it is probably a struct. so move the atomicR to some defn ctrlBlockR *)
-  Definition SharedPtrR (cppty: type) (id: CtrlBlockId) (Rpiece : nat -> Rep) (ownedPtr:ptr)  : Rep :=
-    structR ("std::shared_ptr".<<Atype cppty>>) 1
+  Definition SharedPtrR (id: CtrlBlockId) (Rpiece : nat -> Rep) (ownedPtr:ptr)  : Rep :=
+    structR ("std::shared_ptr".<<Atype ty>>) 1
     ** [| ([∗ list] ctid ∈ allContenderIds, Rpiece ctid) |-- anyR "int" 1 |]
-    ** ownedPtrOffset |-> primR (Tptr cppty) 1 (Vptr ownedPtr)
-    ** ctrlBlockPtrOffset |-> primR (Tnamed ("std::atomic".<<Atype "long">>)) 1 (Vptr (dataLoc id))
+    ** ownedPtrOffset |-> primR (Tptr ty) 1 (Vptr ownedPtr)
+    ** ctrlBlockPtrOffset |-> primR (Tptr (Tnamed ("std::atomic".<<Atype "long">>))) 1 (Vptr (dataLoc id))
     ** [| ownedPtr<>nullptr |] (* use NullSharedPtr othewise *)
     ** [| lengthN (contenderLocs id) = Npos maxContention |]
     ** pureR (inv nroot (Exists (ctrVal:N) (pieceOut : nat ->bool) ,
@@ -92,20 +66,13 @@ Section specs.
          ** [| countLN pieceOut allContenderIds  = ctrVal |]
          ** (if (bool_decide (ctrVal = 0))
               then emp
-              else dynAllocatedR cppty ownedPtr))).
+              else dynAllocatedR ty ownedPtr))).
 
-  Definition NullSharedPtrR (cppty: type) : Rep :=
+  Definition NullSharedPtrR : Rep :=
     structR "shared_ptr<int>" 1
-    ** ownedPtrOffset |-> primR (Tptr "cppty") 1 (Vptr nullptr)
-    ** ctrlBlockPtrOffset |->  primR (Tptr "cppty") 1 (Vptr nullptr).
+    ** ownedPtrOffset |-> primR (Tptr ty) 1 (Vptr nullptr)
+    ** ctrlBlockPtrOffset |->  primR (Tptr (Tnamed ("std::atomic".<<Atype "long">>))) 1 (Vptr nullptr).
 
-
-  Definition Lstar (l: list mpred) : mpred := [∗ list] i ∈ l, i.
-
-  Definition allButFirstContenderId := (seq 1 (Pos.to_nat maxContention -1 )).
-
-  Section ty.
-  Context {ty:type}.
 
   Definition init_ctor :=
     specify {| info_name := (Nscoped ("std::shared_ptr".<<Atype ty>>) (Nctor [Tptr ty])).<<Atype ty, Atype "void">>
@@ -119,29 +86,20 @@ Section specs.
     (*           ^^ if anyR is not meaningful for non-scalar types,
                  replace this with wp of default destructor *)
     \post Exists (ctrlBlockId: CtrlBlockId),
-       this |-> SharedPtrR "int"  ctrlBlockId Rpiece p
+       this |-> SharedPtrR ctrlBlockId Rpiece p
        ** ([∗ list] ctid ∈ allButFirstContenderId, copyConstrRight ctrlBlockId ctid)).
 
   Definition SpecFor_init_ctor := RegisterSpec init_ctor.
   #[global] Existing Instance SpecFor_init_ctor.
 
-  
-
-  (** move constructor. the new object represents the same piece of ownership 
-  cpp.spec "std::shared_ptr<int>::shared_ptr(std::shared_ptr<int>&&)" as shm with (fun (this:ptr) =>
-    \arg{other:ptr} "other" (Vptr other)
-    \pre{ctrlBlockId ownedPtr Rpiece} other |-> SharedPtrR "int" ctrlBlockId Rpiece ownedPtr
-    \post other  |-> NullSharedPtrR "int"
-          ** this |-> SharedPtrR "int"  ctrlBlockId Rpiece ownedPtr).
- *)
   Notation spty := ("std::shared_ptr".<<Atype ty>>).
   Definition move_ctor :=
     specify.template.ctor spty [Trv_ref ((Tnamed spty))] $
     \this this
     \arg{other:ptr} "other" (Vptr other)
-    \pre{ctrlBlockId ownedPtr Rpiece} other |-> SharedPtrR ty ctrlBlockId Rpiece ownedPtr
-    \post other  |-> NullSharedPtrR "int"
-          ** this |-> SharedPtrR "int"  ctrlBlockId Rpiece ownedPtr.
+    \pre{ctrlBlockId ownedPtr Rpiece} other |-> SharedPtrR ctrlBlockId Rpiece ownedPtr
+    \post other  |-> NullSharedPtrR
+          ** this |-> SharedPtrR ctrlBlockId Rpiece ownedPtr.
 
   Definition SpecFor_move_ctor := RegisterSpec move_ctor.
   #[global] Existing Instance SpecFor_move_ctor.
@@ -152,9 +110,9 @@ Section specs.
     \pre{(null:bool) (p:ptr) (sid: if null then unit else prod CtrlBlockId nat) Rpiece}
       this |-> (match null as b return (if b then unit else prod CtrlBlockId nat) -> Rep with
                 | false => fun sid=>
-                             SharedPtrR "int" sid.1 Rpiece p
+                             SharedPtrR sid.1 Rpiece p
                              ** Rpiece sid.2
-                | true => fun sid=> NullSharedPtrR "int"
+                | true => fun sid=> NullSharedPtrR
                 end) sid
 
     \post (match null as b return (if b then unit else prod CtrlBlockId nat) -> mpred with
@@ -165,39 +123,17 @@ Section specs.
   Definition SpecFor_dtor := RegisterSpec dtor_spec.
   #[global] Existing Instance SpecFor_dtor.
 
-  (*
-  cpp.spec "std::shared_ptr<int>::~shared_ptr()" as shd1 with (fun (this:ptr) =>
-    \with (null:bool)
-    \pre{(p:ptr) (sid: if null then unit else prod CtrlBlockId nat) Rpiece}
-      this |-> (match null as b return (if b then unit else prod CtrlBlockId nat) -> Rep with
-                | false => fun sid=>
-                             SharedPtrR "int" sid.1 Rpiece p
-                             ** Rpiece sid.2
-                | true => fun sid=> NullSharedPtrR "int"
-                end) sid
-
-    \post (match null as b return (if b then unit else prod CtrlBlockId nat) -> mpred with
-                | false => fun sid=> copyConstrRight sid.1 sid.2
-                | true => fun sid=> emp
-                end) sid).
- *)
-  (*
-  cpp.spec "std::shared_ptr<int>::~shared_ptr()" as shd2 with (fun (this:ptr) =>
-    \pre this |-> NullSharedPtrR "int"
-    \post emp).
-  *)
-
 
   Definition copy_ctor :=
     specify.template.ctor spty [Tref (Tconst (Tnamed spty))] $
     \this this
     \arg{other:ptr} "other" (Vptr other)
     \pre{id ctid p Rpiece}
-         other |-> SharedPtrR "int" id Rpiece p
+         other |-> SharedPtrR id Rpiece p
          ** copyConstrRight id ctid (* this will be returned by destructor *)
     \post
-         p|->Rpiece ctid ** this  |-> SharedPtrR "int" id Rpiece p
-          ** other |-> SharedPtrR "int" id Rpiece p.
+         p|->Rpiece ctid ** this  |-> SharedPtrR id Rpiece p
+          ** other |-> SharedPtrR id Rpiece p.
                           
   Definition SpecFor_copy_ctor := RegisterSpec copy_ctor.
   #[global] Existing Instance SpecFor_copy_ctor.
@@ -209,11 +145,11 @@ Section specs.
     \this this
     \arg{other:ptr} "other" (Vptr other)
     \pre{id ctid p Rpiece}
-         other |-> SharedPtrR "int" id Rpiece p
+         other |-> SharedPtrR id Rpiece p
          ** copyConstrRight id ctid (* this will be returned by destructor *)
     \post
-         p|->Rpiece ctid ** this  |-> SharedPtrR "int" id Rpiece p
-          ** other |-> SharedPtrR "int" id Rpiece p.
+         p|->Rpiece ctid ** this  |-> SharedPtrR id Rpiece p
+          ** other |-> SharedPtrR id Rpiece p.
 
 
   Definition SP_acc  := ("std::__shared_ptr_access" .<< 
@@ -232,31 +168,24 @@ Section specs.
   Definition upcast_offset : offset :=
     (o_derived σ SP_acc SP_impl ,, o_derived σ SP_impl SP).
 
-  (*
-  cpp.spec (SP_acc.::Nop function_qualifiers.Nc OOStar []) as shg with 
-    (fun (this:ptr) =>
-       \prepost{id p Rpiece} this |-> upcast_offset |-> SharedPtrR "int" id Rpiece p
-       \post[Vptr p] emp
-       ).
-*)
   Definition deref :=
     specify.template.op SP_acc OOStar function_qualifiers.Nc (Tref ty) [] $
        \this this
-       \prepost{id p Rpiece} this |-> upcast_offset |-> SharedPtrR "int" id Rpiece p
+       \prepost{id p Rpiece} this |-> upcast_offset |-> SharedPtrR id Rpiece p
        \post[Vref p] emp.
 
   Definition SpecFor_deref := RegisterSpec deref.
   #[global] Existing Instance SpecFor_deref.
   
-  #[global] Instance sharedR_typeptr_observe ty id (p:ptr) op Rpiece
-    : Observe (type_ptr (Tnamed ("std::shared_ptr".<<Atype ty>>)) p) (p|->SharedPtrR ty id Rpiece op):= _.
+  #[global] Instance sharedR_typeptr_observe id (p:ptr) op Rpiece
+    : Observe (type_ptr (Tnamed ("std::shared_ptr".<<Atype ty>>)) p) (p|->SharedPtrR id Rpiece op):= _.
   
 
   Definition allPiecesAndObjs Rpiece id (ownedPtr: ptr) (pieceOut: nat->bool) : Rep :=
    ([∗ list] ctid ∈ allContenderIds,
      if pieceOut ctid
      then pureR (ownedPtr |-> Rpiece ctid)
-          ** SharedPtrR "int" id Rpiece ownedPtr
+          ** SharedPtrR id Rpiece ownedPtr
      else pureR (copyConstrRight id ctid)).
 
   Lemma redistributePayloadOwnership {Rpieceold Rpiecenew: nat -> Rep} (pieceOut : nat -> bool) id ownedPtr:
@@ -264,23 +193,28 @@ Section specs.
       |-- allPiecesAndObjs Rpiecenew id ownedPtr pieceOut.
   Proof. Admitted.
 
-  cpp.spec "testnew4()" as testnew4spec with (
-    \pre emp
-    \post{p:ptr}[Vptr p] Exists payload sid,
-       p |-> SharedPtrR "int" sid (fun ctid => if bool_decide (ctid=0%nat) then anyR "int" 1 else emp) payload
-       ** payload |-> intR (cQp.m 1) 1
-       ** ([∗ list] ctid ∈ allButFirstContenderId,
-              copyConstrRight sid ctid)
-    ).
+
+End specs.
 
 
+Hint Resolve NoDup_seq : setsolver.
+Hint Rewrite elem_of_seq: equiv.
+Hint Rewrite @big_sepL_emp: equiv.
+
+Lemma seqprefix (prelen len start: nat):
+  (prelen <= len)%nat -> seq start len = (seq start prelen)++(seq (start+prelen) (len -prelen)).
+Proof using.
+  intros Hl.
+  replace len with (prelen+(len-prelen))%nat at 1 by lia.
+  rewrite seq_app.
+  reflexivity.
+Qed.
   
 Lemma one_as_bigsep {PROP: bi} {A} {eqd: EqDecision A} (f  : PROP) l (x: A):
   x ∈ l ->
   NoDup l -> (* too strong: we only need x to be not duplicated *)
   f -|- ([∗ list] id ∈ l, if bool_decide (id=x) then f else emp)%I.
 Proof using.
-  clear MOD.
   intros.
   rewrite  -> big_op.big_sepL_difference_singleton with (x:=x) by assumption.
   simpl.
@@ -301,34 +235,45 @@ Proof using.
   set_solver.
 Qed.
 
-Hint Resolve NoDup_seq : setsolver.
-Hint Rewrite elem_of_seq: equiv.
-Hint Rewrite @big_sepL_emp: equiv.
-Lemma allButFirstEmp : ([∗ list] x ∈ seq 1 (Pos.to_nat maxContention -1), 
+Section proofs.
+  (** proofs: *)
+  Opaque SharedPtrR.
+  Context `{Σ : cpp_logic, MOD:inc_shared_ptr_cpp.module ⊧ σ}
+  {hf:fracG () _Σ} (ty:type).
+  
+  Definition observeSharedType r q t Rpiece op:= @observe_fwd _ _ _ (sharedR_typeptr_observe r q t Rpiece op).
+
+  cpp.spec "testnew4()" as testnew4spec with (
+    \pre emp
+    \post{p:ptr}[Vptr p] Exists payload sid,
+       p |-> SharedPtrR "int" sid (fun ctid => if bool_decide (ctid=0%nat) then anyR "int" 1 else emp) payload
+       ** payload |-> intR (cQp.m 1) 1
+       ** ([∗ list] ctid ∈ allButFirstContenderId,
+              copyConstrRight sid ctid)
+    ).
+
+
+
+  Lemma allButFirstEmp : ([∗ list] x ∈ seq 1 (Pos.to_nat maxContention -1), 
        if bool_decide (x = 0%nat)
        then anyR "int" 1$m
        else emp)
                          -|- emp.
-Proof using.
-  erewrite  big_opL_proper with (g := fun _ _=> emp).
-  2:{ intros ? ? Hl.
-      apply elem_of_list_lookup_2 in Hl.
-      autorewrite with equiv in Hl.
-      resolveDecide lia.
-      reflexivity.
-  }
-  autorewrite with equiv.
-  reflexivity.
-Qed.
-
-End ty.
-  (** proofs: *)
-  Opaque SharedPtrR.
+  Proof using.
+    erewrite  big_opL_proper with (g := fun _ _=> emp).
+    2:{ intros ? ? Hl.
+        apply elem_of_list_lookup_2 in Hl.
+        autorewrite with equiv in Hl.
+        resolveDecide lia.
+        reflexivity.
+    }
+    autorewrite with equiv.
+    reflexivity.
+  Qed.
   
-  Definition observeSharedType r q t Rpiece op:= @observe_fwd _ _ _ (sharedR_typeptr_observe r q t Rpiece op).
-
   Opaque NullSharedPtrR.
   Hint Resolve observeSharedType : br_opacity.
+  Print SpecFor_copy_ctor.
   Lemma prf2: verify[module] testnew4spec.
   Proof using MOD.
     verify_spec.
@@ -340,7 +285,6 @@ End ty.
     iExists Rpiece.
     go.
     iExists _.
-    iExists 0.
     simpl.
     eagerUnifyU.
     go.
@@ -376,6 +320,4 @@ End ty.
     iExists Rpiece.
     ego.
   Qed.
-  
-  Disable Notation "::wpOperand".
-End specs.
+End proofs.
